FOL_Compactness/Skolem_Normal_Form.thy
@@ -34,11 +34,11 @@ proof -
   next
     case (Fun f ts)
     then have \<open>u \<in> set ts \<Longrightarrow> \<lbrakk>u\<rbrakk>\<^bsup>I,\<beta>\<^esup> \<in> dom I\<close> for u
-      by (smt (z3) UN_iff Un_iff eq_fst_iff functions_term.simps(2) is_interpretation_def)
+      by (smt (verit) UN_I Un_iff fst_conv funas_term.simps(2) is_interpretation_def list.set_map)
     then show ?case
       using eval.simps(2) fst_conv imageE length_map list.set_map list_all_set assms(2)
       unfolding is_valuation_def
-      by (smt (verit, best) Fun.prems Un_insert_left functions_term.simps(2) insert_iff 
+      by (smt (verit, best) Fun.prems Un_insert_left funas_term.simps(2) insert_iff 
           is_interpretation_def subsetI)
   qed
   ultimately have \<open>\<exists>a \<in> dom I. I\<^bold>, \<beta>(x := a) \<Turnstile> \<phi>\<close>
@@ -122,7 +122,7 @@ next
   case (2 p ts)
   then show ?case
     by (metis (no_types, lifting) UnCI eval_term.simps(1) formsubst_functions_form 
-        functions_term.simps(2) mem_Collect_eq singletonI subst_simps(1))
+        funas_term.simps(2) mem_Collect_eq singletonI subst_simps(1))
 next
   case (3 \<phi> \<psi>)
   then show ?case
@@ -131,7 +131,7 @@ next
   case (4 y \<phi>)
   then show ?case
     by (metis (no_types, lifting) UnI2 Un_commute eval_term.simps(1) formsubst_functions_form 
-        functions_term.simps(2) mem_Collect_eq singletonI subst_simps(1))
+        funas_term.simps(2) mem_Collect_eq singletonI subst_simps(1))
 qed
 
 (* the following lemmas may be useful*)
